CircuitTest.dfy
@@ -1,0 +1,54 @@
+module CircuitTest {
+
+    import opened Std.Wrappers
+    import C = Circuit
+    import P = Primitives
+    // Make a circuit with a single XOR gate.
+
+    function behav_xor(inputs: map<C.CPort, bool>): Option<map<C.CPort, bool>>
+    {
+        if 0 !in inputs then
+            None
+        else if 1 !in inputs then
+            None
+        else
+            var o := if inputs[0] == inputs[1] then false else true;
+            Some(map[2 := o])
+    }
+
+    const circ := C.Circuit(
+        NodeKind := (n: C.CNode) => (match n
+            case 0 => Some(C.CInput())
+            case 1 => Some(C.CInput())
+            case 2 => Some(C.COutput())
+            case 3 => Some(P.nk_xor)
+            case _ => None
+            ),
+        PortSource := (np: C.NP) => (match np
+            case NP(3, 0) => Some(C.NP(0, 1))
+            case NP(3, 1) => Some(C.NP(1, 1))
+            case NP(2, 0) => Some(C.NP(3, 2))
+            case _ => None),
+        PortNames := _ => None,
+        NodeBound := 4,
+        PortBound := 3,
+        HierLevel := 0
+    )
+    const lib := C.CLib([circ])
+
+    const HierLevel: nat := 0
+    const PortBound: C.CPort := 4
+
+    lemma nk_xor_valid()
+        ensures C.CNodeKindValid(lib, HierLevel, PortBound, nk_xor)
+    {
+        reveal C.CircuitValid();
+    }
+
+    lemma CircValid()
+        ensures C.CircuitValid(lib, circ)
+    {
+        reveal C.CircuitValid();
+    }
+
+}
