Primitives.dfy
@@ -1,0 +1,30 @@
+module Primitives {
+
+    import opened Std.Wrappers
+    import C = Circuit
+
+    function behav_xor(inputs: map<C.CPort, bool>): Option<map<C.CPort, bool>>
+    {
+        if 0 !in inputs then
+            None
+        else if 1 !in inputs then
+            None
+        else
+            var o := if inputs[0] == inputs[1] then false else true;
+            Some(map[2 := o])
+    }
+
+    const nk_xor := C.CComb(
+        IPorts := {0, 1},
+        OPorts := {2},
+        PathExists := (a: C.CPort, b: C.CPort) => (
+            match (a, b)
+            case (2, 0) => true
+            case (2, 1) => true
+            case _ => false
+        ),
+        Behav := behav_xor,
+        PortNames := C.PortNames2to1
+    )
+
+}
